lithium tutorial

src/Iris/Examples/Exp.lean
@@ -7,57 +7,76 @@ import Iris.BI
 import Iris.ProofMode
 
 namespace Iris.Examples.Lang
-open BI
-
-variable {u} [BI.{u} PROP]
 
 inductive Binder where
 | anon : Binder
 | str : String → Binder
-deriving Inhabited, BEq, Repr
+deriving DecidableEq, Inhabited, Repr
 
 instance : Coe String Binder where
   coe := Binder.str
 
 def Loc : Type := Nat
+deriving DecidableEq
 
 inductive Binop where
-| plus | minus | eq
+| plus | minus | eq | pair
+deriving DecidableEq
 
 mutual
 inductive Val where
 | nat : Nat -> Val
 | loc : Loc -> Val
+| pair : Val -> Val -> Val
 | recv : Binder -> Binder -> Exp -> Val
+deriving DecidableEq
 inductive Exp where
 | val : Val -> Exp
 | var : String -> Exp
 | binop : Exp -> Binop -> Exp -> Exp
+| fst : Exp -> Exp
+| snd : Exp -> Exp
 | rece : Binder -> Binder -> Exp -> Exp
 | lete : Binder -> Exp -> Exp -> Exp
 | app : Exp -> Exp -> Exp
 | ife : Exp -> Exp -> Exp -> Exp
+| alloc : Exp
+| load : Exp -> Exp
+| store : Exp -> Exp -> Exp
+deriving DecidableEq
 end
 
 def subst (x : String) (v : Val) : Exp → Exp
   | .val v => .val v
   | .var y => if x == y then .val v else .var y
   | .binop e1 o e2 => .binop (subst x v e1) o (subst x v e2)
+  | .fst e1 => .fst (subst x v e1)
+  | .snd e1 => .snd (subst x v e1)
   | .rece f y e' => .rece f y (if .str x == f || .str x == y then e' else subst x v e')
   | .lete y e1 e2 => .lete y (subst x v e1) (if .str x == y then e2 else subst x v e2)
   | .app e1 e2 => .app (subst x v e1) (subst x v e2)
   | .ife e1 e2 e3 => .ife (subst x v e1) (subst x v e2)  (subst x v e3)
+  | .alloc => .alloc
+  | .load e1 => .load (subst x v e1)
+  | .store e1 e2 => .store (subst x v e1) (subst x v e2)
 
 def subst' (x : Binder) (v : Val) (e : Exp) : Exp :=
   match x with
   | .anon => e
   | .str x => subst x v e
 
+
+section wp
+open BI
+
+variable {u} [BI.{u} PROP]
 def wp [BI PROP] (e : Exp) (P : Val -> PROP) : PROP := by sorry
 
 theorem wp_wand e (P1 P2 : Val -> PROP) :
   ⊢ wp e P1 -∗ (∀ v, P1 v -∗ P2 v) -∗ wp e P2
   := by sorry
+
+end wp
 
 namespace Reify
 open Lean
@@ -65,10 +84,15 @@ inductive Exp where
 | val : Expr -> Exp -- we do not need to reify values
 | var : String -> Exp
 | binop : Exp -> Expr -> Exp -> Exp
+| fst : Exp -> Exp
+| snd : Exp -> Exp
 | rece : Binder -> Binder -> Exp -> Exp
 | lete : Binder -> Exp -> Exp -> Exp
 | app : Exp -> Exp -> Exp
 | ife : Exp -> Exp -> Exp -> Exp
+| alloc : Exp
+| load : Exp -> Exp
+| store : Exp -> Exp -> Exp
 | unk : Expr -> Exp
 deriving Inhabited, Repr
 
@@ -82,10 +106,15 @@ def Exp.unreify : Exp → Expr
   | .val v => mkApp (mkConst ``Lang.Exp.val) v
   | .var v => mkApp (mkConst ``Lang.Exp.var) (mkStrLit v)
   | .binop e1 o e2 => mkApp3 (mkConst ``Lang.Exp.binop) (unreify e1) o (unreify e2)
+  | .fst e1 => mkApp (mkConst ``Lang.Exp.fst) (unreify e1)
+  | .snd e1 => mkApp (mkConst ``Lang.Exp.snd) (unreify e1)
   | .rece f x e => mkApp3 (mkConst ``Lang.Exp.rece) (Binder.unreify f) (Binder.unreify x) (unreify e)
   | .lete x e1 e2 => mkApp3 (mkConst ``Lang.Exp.lete) (Binder.unreify x) (unreify e1) (unreify e2)
   | .app e1 e2 => mkApp2 (mkConst ``Lang.Exp.app) (unreify e1) (unreify e2)
   | .ife e1 e2 e3 => mkApp3 (mkConst ``Lang.Exp.ife) (unreify e1) (unreify e2) (unreify e3)
+  | .alloc => mkConst ``Lang.Exp.alloc
+  | .load e1 => mkApp (mkConst ``Lang.Exp.load) (unreify e1)
+  | .store e1 e2 => mkApp2 (mkConst ``Lang.Exp.store) (unreify e1) (unreify e2)
   | .unk e => e
 
 def Binder.reify (e : Expr) : Option Binder :=
@@ -105,6 +134,8 @@ partial def reify (e : Expr) : Exp :=
     | .lit (.strVal v) => .var v
     | _ => .unk e
   | Lang.Exp.binop e1 o e2 => .binop (reify e1) o (reify e2)
+  | Lang.Exp.fst e1 => .fst (reify e1)
+  | Lang.Exp.snd e1 => .snd (reify e1)
   | Lang.Exp.rece f x e' =>
     match Binder.reify f, Binder.reify x with
     | some f, some x => .rece f x (reify e')
@@ -115,6 +146,9 @@ partial def reify (e : Expr) : Exp :=
     | _ => .unk e
   | Lang.Exp.app e1 e2 => .app (reify e1) (reify e2)
   | Lang.Exp.ife e1 e2 e3 => .ife (reify e1) (reify e2) (reify e3)
+  | Lang.Exp.alloc => .alloc
+  | Lang.Exp.load e1 => .load (reify e1)
+  | Lang.Exp.store e1 e2 => .store (reify e1) (reify e2)
   | _ => .unk e
 
 def subst (x : String) (v : Expr) (e : Exp) : Exp :=
@@ -122,10 +156,15 @@ def subst (x : String) (v : Expr) (e : Exp) : Exp :=
   | .val _ => e
   | .var y => if x == y then .val v else e
   | .binop e1 o e2 => .binop (subst x v e1) o (subst x v e2)
+  | .fst e1 => .fst (subst x v e1)
+  | .snd e1 => .snd (subst x v e1)
   | .rece f y e' => .rece f y (if .str x == f || .str x == y then e' else subst x v e')
   | .lete y e1 e2 => .lete y (subst x v e1) (if .str x == y then e2 else subst x v e2)
   | .app e1 e2 => .app (subst x v e1) (subst x v e2)
   | .ife e1 e2 e3 => .ife (subst x v e1) (subst x v e2)  (subst x v e3)
+  | .alloc => .alloc
+  | .load e1 => .load (subst x v e1)
+  | .store e1 e2 => .store (subst x v e1) (subst x v e2)
   | .unk e => .unk (mkApp3 (mkConst ``Lang.subst) (mkStrLit x) v e)
 
 def subst' (x : Binder) (v : Expr) (e : Exp) : Exp :=
